Use {{..}} in simp rules

Denotational.thy
@@ -8,7 +8,7 @@ where
   "atom x \<sharp> \<rho> ==> \<lbrakk> Lam [x]. e \<rbrakk>\<^bsub>\<rho>\<^esub> = Fn \<cdot> (\<Lambda> v. (\<lbrakk> e \<rbrakk>\<^bsub>\<rho>(x f\<mapsto> v)\<^esub>))"
 | "\<lbrakk> App e x \<rbrakk>\<^bsub>\<rho>\<^esub> = \<lbrakk> e \<rbrakk>\<^bsub>\<rho>\<^esub> \<down>Fn \<lbrakk> Var x \<rbrakk>\<^bsub>\<rho>\<^esub> "
 | "\<lbrakk> Var x \<rbrakk>\<^bsub>\<rho>\<^esub> = the (lookup \<rho> x)"
-| "set (bn as) \<sharp>* \<rho> \<Longrightarrow>\<lbrakk> Let as body\<rbrakk>\<^bsub>\<rho>\<^esub> = \<lbrakk>body\<rbrakk>\<^bsub>heapExtend \<rho> (asToHeap as) ESem\<^esub>"
+| "set (bn as) \<sharp>* \<rho> \<Longrightarrow>\<lbrakk>Let as body\<rbrakk>\<^bsub>\<rho>\<^esub> = \<lbrakk>body\<rbrakk>\<^bsub>heapExtend \<rho> (asToHeap as) ESem\<^esub>"
 proof-
 case goal1 thus ?case
   unfolding eqvt_def ESem_graph_def
@@ -112,6 +112,7 @@ lemma  True and [simp]:"(a, b) \<in> set (asToHeap as) \<Longrightarrow> size b 
 
 termination (eqvt) by lexicographic_order
 
+
 lemma ESem_cont':"Y0 = Y 0 \<Longrightarrow> chain Y \<Longrightarrow> range (\<lambda>i. \<lbrakk> e \<rbrakk>\<^bsub>Y i\<^esub>) <<| \<lbrakk> e \<rbrakk>\<^bsub>(\<Squnion> i. Y i)\<^esub> " and True
 proof(nominal_induct e and avoiding: Y0  arbitrary: Y rule:exp_assn.strong_induct)
 case (Lam x e Y0 Y)
@@ -148,5 +149,17 @@ qed simp
 
 lemma ESem_cont: "cont (ESem e)"  using ESem_cont'[OF refl] by (rule contI)
 
+lemmas ESem_cont2cont[simp,cont2cont] = cont_compose[OF ESem_cont]
+
+
+definition HSem ("\<lbrace>_\<rbrace>_"  [60,60] 60) where "\<lbrace>\<Gamma>\<rbrace>\<rho> = heapExtend \<rho> \<Gamma> ESem"
+
+lemma Esem_simps4[simp]: "set (bn as) \<sharp>* \<rho> \<Longrightarrow> \<lbrakk> Terms.Let as body \<rbrakk>\<^bsub>\<rho>\<^esub> = \<lbrakk> body \<rbrakk>\<^bsub>\<lbrace>asToHeap as \<rbrace>\<rho>\<^esub>"
+  by (simp add: HSem_def)
+
+lemma HSem_def': "\<lbrace>\<Gamma>\<rbrace>\<rho> = fmap_update \<rho> (fix1 (fmap_bottom (fst ` set \<Gamma>)) (\<Lambda> \<rho>'. heapToEnv \<Gamma> (\<lambda>e. \<lbrakk>e\<rbrakk>\<^bsub>fmap_update \<rho> \<rho>'\<^esub>))) "
+  unfolding HSem_def heapExtend_def by simp
+
+declare ESem.simps(4)[simp del]
 
 end
